Cleanup

Union_Find_Time_alpha_verification.thy
@@ -320,16 +320,16 @@ definition is_uf2 :: "(nat\<times>nat) set \<Rightarrow> uf \<Rightarrow> assn" 
   "is_uf2 R u \<equiv> case u of (s,p) \<Rightarrow> 
   \<exists>\<^sub>Al rkl. p\<mapsto>\<^sub>al * s\<mapsto>\<^sub>arkl 
     * \<up>(ufa_\<alpha> l = R \<and> length rkl = length l \<and> invar_rank l rkl)
-    * $(\<Phi> l rkl * 10)"
+    * $(\<Phi> l rkl * 4)"
 
 thm ufa_\<alpha>_dom_card
 
 subsubsection{*uf_cmp lemmas*}
 
-definition uf_cmp_time where "uf_cmp_time n \<equiv> 2 * uf_rep_of_c_time n + 10"
+definition uf_cmp_time where "uf_cmp_time n \<equiv> 8 * uf_rep_of_c_time n + 40"
 
 lemma uf_cmp_rule: "\<lbrakk>invar_rank l rkl\<rbrakk> \<Longrightarrow>
-  <p\<mapsto>\<^sub>al * $(4*(\<Phi> l rkl + uf_cmp_time (length l)) )> 
+  <p\<mapsto>\<^sub>al * $(4*\<Phi> l rkl + uf_cmp_time (length l) )> 
   uf_cmp (s,p) i j 
   <\<lambda>r.\<exists>\<^sub>A l'. p\<mapsto>\<^sub>al' 
     *$(4* \<Phi> l' rkl) * \<up>((r\<longleftrightarrow>(rep_of l i = rep_of l j)) \<and> invar_rank l' rkl
@@ -341,92 +341,91 @@ proof goal_cases
         (8 * uf_rep_of_c_time (length l) + 40) = 4 * \<Phi> l rkl +
         (8 * uf_rep_of_c_time (length l) + 39) + 1" by algebra
   from 1 show ?case
-unfolding uf_cmp_time_def uf_cmp_def
-  apply vcg
-  apply simp
-  apply (subst sum1) apply (subst time_credit_add[of "(4 * \<Phi> l rkl +
+    unfolding uf_cmp_time_def uf_cmp_def
+    apply vcg
+     apply (subst sum1) apply (subst time_credit_add[of "(4 * \<Phi> l rkl +
         (8 * uf_rep_of_c_time (length l) + 39))" 1])
-  apply (sep_auto heap: length_rule)
-  apply safe proof goal_cases
-  case (1 x)
-  then show ?case 
-  proof (cases "x \<le> i \<or> x \<le> j")
-    case True
-    then show ?thesis using 1 apply vcg 
-    proof goal_cases
-      case (1 x')
-      hence " p \<mapsto>\<^sub>a l *
+     apply (sep_auto heap: length_rule)
+    apply safe proof goal_cases
+    case (1 x)
+    then show ?case 
+    proof (cases "x \<le> i \<or> x \<le> j")
+      case True
+      then show ?thesis using 1 apply vcg 
+      proof goal_cases
+        case (1 x')
+        hence " p \<mapsto>\<^sub>a l *
     $ (\<Phi> l rkl * 4 + uf_rep_of_c_time (length l) * 8 + 38) *
     \<up> (\<not> x') \<Longrightarrow>\<^sub>A p \<mapsto>\<^sub>a l * true * $ (4 * \<Phi> l rkl) *
        \<up> (x' = (rep_of l i = rep_of l j) \<and>
           invar_rank l rkl \<and>
           length l = length l \<and>
           (\<forall>i<length l. rep_of l i = rep_of l i))"  sorry
-      then show ?case  using ent_ex_postI by fast
-    qed
-next
-  case False
-  have sum2: "\<Phi> l rkl * 4 + uf_rep_of_c_time (length l) * 8 + 39 
+        then show ?case  using ent_ex_postI by fast
+      qed
+    next
+      case False
+      have sum2: "\<Phi> l rkl * 4 + uf_rep_of_c_time (length l) * 8 + 39 
             = \<Phi> l rkl * 4 + uf_rep_of_c_time (length l) * 4 + uf_rep_of_c_time (length l) * 4 + 39" 
-    by algebra
-  have sep2: "$(\<Phi> l rkl * 4 + uf_rep_of_c_time (length l) * 4 +
+        by algebra
+      have sep2: "$(\<Phi> l rkl * 4 + uf_rep_of_c_time (length l) * 4 +
             uf_rep_of_c_time (length l) * 4 +
             39)  =   $ (\<Phi> l rkl * 4 + uf_rep_of_c_time (length l) * 4) * 
             $ (uf_rep_of_c_time (length l) * 4 + 39)"
-    using time_credit_add add.assoc[of "\<Phi> l rkl * 4 + uf_rep_of_c_time (length l) * 4" 
-          "uf_rep_of_c_time (length l) * 4" 39] by presburger
+        using time_credit_add add.assoc[of "\<Phi> l rkl * 4 + uf_rep_of_c_time (length l) * 4" 
+            "uf_rep_of_c_time (length l) * 4" 39] by presburger
 
-  also have sep3: "\<dots> =    $ (4* (\<Phi> l rkl + uf_rep_of_c_time (length l))) * 
+      also have sep3: "\<dots> =    $ (4* (\<Phi> l rkl + uf_rep_of_c_time (length l))) * 
             $ (uf_rep_of_c_time (length l) * 4 + 39)" 
-    by (simp add: mult.commute)
-  have sep4: "p \<mapsto>\<^sub>a l *
+        by (simp add: mult.commute)
+      have sep4: "p \<mapsto>\<^sub>a l *
          ($ (4 * (\<Phi> l rkl + uf_rep_of_c_time (length l))) *
           $ (uf_rep_of_c_time (length l) * 4 + 39)) = p \<mapsto>\<^sub>a l *
    $ (4 * (\<Phi> l rkl + uf_rep_of_c_time (length l))) *
    $ (uf_rep_of_c_time (length l) * 4 + 39 )" by simp
-  have "i<x" "j<x" using False by auto
-  with \<open>invar_rank l rkl\<close> show ?thesis apply auto apply vcg 
-    apply (subst sum2)
-     apply (subst sep2)
-     apply (subst sep3)
-     apply (subst sep4)
-    apply (rule frame_rule[of "p \<mapsto>\<^sub>a l * $ (4 * (\<Phi> l rkl + uf_rep_of_c_time (length l)))" "uf_rep_of_c p i"
-                   _ "$ (uf_rep_of_c_time (length l) * 4 + 39)" ] )
-     apply (vcg heap: uf_rep_of_c_rule''' )
-    apply vcg apply auto proof goal_cases
-    case (1 x')
-    then show ?case apply (vcg (ss)) apply (vcg (ss)) 
-    proof goal_cases
-      case (1 l')
-      hence inv:"invar_rank l' rkl" by blast
-      from 1 have ll': "length l = length l'" by argo
-      have sum3: "4 * \<Phi> l' rkl + (uf_rep_of_c_time (length l) * 4 + 39) = 4 * (\<Phi> l' rkl +
-        (uf_rep_of_c_time (length l))) + 39" by algebra
-      have sep5: "p \<mapsto>\<^sub>a l' * true * $ (4 * (\<Phi> l' rkl + uf_rep_of_c_time (length l')) + 39) 
-                = p \<mapsto>\<^sub>a l' *        $ (4 * (\<Phi> l' rkl + uf_rep_of_c_time (length l'))) * ($(39) * true)"        
-        by (simp add: time_credit_add)
-      from 1 ll' inv show ?case apply (subst sum3) apply (subst (asm) ll')+ apply (subst ll')+
-        apply vcg apply (subst sep5)
-        apply (rule frame_rule[of "p \<mapsto>\<^sub>a l' * $ (4 * (\<Phi> l' rkl + uf_rep_of_c_time (length l')))"
-             "uf_rep_of_c p j" _ " ($ 39 * true)"])
+      have "i<x" "j<x" using False by auto
+      with \<open>invar_rank l rkl\<close> show ?thesis apply auto apply vcg 
+         apply (subst sum2)
+         apply (subst sep2)
+         apply (subst sep3)
+         apply (subst sep4)
+         apply (rule frame_rule[of "p \<mapsto>\<^sub>a l * $ (4 * (\<Phi> l rkl + uf_rep_of_c_time (length l)))" "uf_rep_of_c p i"
+              _ "$ (uf_rep_of_c_time (length l) * 4 + 39)" ] )
          apply (vcg heap: uf_rep_of_c_rule''' )
-        apply vcg
-        apply auto
-        apply vcg
-        apply auto proof goal_cases
-        case (1 l'')
-        have "p \<mapsto>\<^sub>a l'' * true * $ (\<Phi> l'' rkl * 4 + 38) \<Longrightarrow>\<^sub>A
+        apply vcg apply auto proof goal_cases
+        case (1 x')
+        then show ?case apply (vcg (ss)) apply (vcg (ss)) 
+        proof goal_cases
+          case (1 l')
+          hence inv:"invar_rank l' rkl" by blast
+          from 1 have ll': "length l = length l'" by argo
+          have sum3: "4 * \<Phi> l' rkl + (uf_rep_of_c_time (length l) * 4 + 39) = 4 * (\<Phi> l' rkl +
+        (uf_rep_of_c_time (length l))) + 39" by algebra
+          have sep5: "p \<mapsto>\<^sub>a l' * true * $ (4 * (\<Phi> l' rkl + uf_rep_of_c_time (length l')) + 39) 
+                = p \<mapsto>\<^sub>a l' *        $ (4 * (\<Phi> l' rkl + uf_rep_of_c_time (length l'))) * ($(39) * true)"        
+            by (simp add: time_credit_add)
+          from 1 ll' inv show ?case apply (subst sum3) apply (subst (asm) ll')+ apply (subst ll')+
+            apply vcg apply (subst sep5)
+             apply (rule frame_rule[of "p \<mapsto>\<^sub>a l' * $ (4 * (\<Phi> l' rkl + uf_rep_of_c_time (length l')))"
+                  "uf_rep_of_c p j" _ " ($ 39 * true)"])
+             apply (vcg heap: uf_rep_of_c_rule''' )
+            apply vcg
+            apply auto
+            apply vcg
+            apply auto proof goal_cases
+            case (1 l'')
+            have "p \<mapsto>\<^sub>a l'' * true * $ (\<Phi> l'' rkl * 4 + 38) \<Longrightarrow>\<^sub>A
   p \<mapsto>\<^sub>a l'' * true * $ (4 * \<Phi> l'' rkl) *
   \<up> (invar_rank l'' rkl \<and>
      length l'' = length l' \<and>
      (\<forall>i<length l'. rep_of l'' i = rep_of l i))" using 1 apply sep_auto
-          by (smt assn_times_assoc gc_time le_add1 match_first merge_true_star mult.commute)
-        then  show ?case using ent_ex_postI by fast 
-      qed
+              by (smt assn_times_assoc gc_time le_add1 match_first merge_true_star mult.commute)
+            then  show ?case using ent_ex_postI by fast 
+          qed
+        qed
+      qed   
     qed
-  qed   
-qed
-qed
+  qed
 qed
 
 
@@ -439,23 +438,12 @@ lemma "  card (Domain (ufa_\<alpha> l)) = length l"
   by simp
 
 
-lemma uf_cmp_rule: "\<lbrakk>invar_rank l rkl\<rbrakk> \<Longrightarrow>
+lemma uf_cmp_rule': "\<lbrakk>invar_rank l rkl\<rbrakk> \<Longrightarrow>
   <is_uf R u * $(uf_cmp_time (card (Domain R)))> uf_cmp u i j <\<lambda>r. is_uf R u * \<up>(r\<longleftrightarrow>(i,j)\<in>R)>\<^sub>t" 
   sorry
   
 
 subsubsection{*uf_union_lemmas*}
-
-
-lemma uf_rep_of_rule_ub: assumes "ufa_invar l" "i<length l"  "invar l szl"
-  shows "<p\<mapsto>\<^sub>al * $(height_ub (length l) + 2)> uf_rep_of p i <\<lambda>r. p\<mapsto>\<^sub>al * \<up>(r=rep_of l i)>\<^sub>t"
-proof -
-  from assms height_ub have "height_of l i \<le> height_ub (length l)" by auto
-  then obtain x where p: "height_ub (length l) = height_of l i + x"  
-    using le_Suc_ex by blast  
-  show ?thesis unfolding p
-    using assms by(sep_auto heap: uf_rep_of_rule)
-qed
 
 
 definition "uf_union_time n = 11+ height_ub n*2"
